src/computational_monads/simulation_semantics/oracle_append.lean
@@ -8,16 +8,16 @@ variables {spec spec' spec'' spec''' : oracle_spec} {A B C : Type}
 
 section oracle_append
 
-def oracle_append' (so : simulation_oracle spec spec'')
-  (so' : simulation_oracle spec' spec''') :
-  simulation_oracle (spec ++ spec') (spec'' ++ spec''') :=
-{
-  S := so.S × so'.S,
-  default_state := (so.default_state, so'.default_state),
-  o := sorry
-}
+-- def oracle_append' (so : simulation_oracle spec spec'')
+--   (so' : simulation_oracle spec' spec''') :
+--   simulation_oracle (spec ++ spec') (spec'' ++ spec''') :=
+-- {
+--   S := so.S × so'.S,
+--   default_state := (so.default_state, so'.default_state),
+--   o := sorry
+-- }
 
-notation so `+++ₛ` so' := oracle_append' so so'
+-- notation so `+++ₛ` so' := oracle_append' so so'
 
 -- TODO: `simulation_oracle.append`
 def oracle_append (so : simulation_oracle spec spec'')
@@ -29,13 +29,14 @@ def oracle_append (so : simulation_oracle spec spec'')
     (λ i, λ x, do { u_s' ← so.o i ⟨x.1, x.2.1⟩, pure (u_s'.1, u_s'.2, x.2.2) })
     (λ i, λ x, do { u_s' ← so'.o i ⟨x.1, x.2.2⟩, pure (u_s'.1, x.2.1, u_s'.2) }) }
 
+-- TODO: should be infix?
 notation so `++ₛ` so' := oracle_append so so'
 
--- Reduce some of the appended oracles independently, and others into a single
-example (so : simulation_oracle spec spec') (so' : simulation_oracle spec' spec')
-  (so'' : simulation_oracle spec'' spec''') :
-  simulation_oracle ((spec ++ spec') ++ spec'') (spec' ++ spec''') :=
-(so ++ₛ so') +++ₛ so''
+-- -- Reduce some of the appended oracles independently, and others into a single
+-- example (so : simulation_oracle spec spec') (so' : simulation_oracle spec' spec')
+--   (so'' : simulation_oracle spec'' spec''') :
+--   simulation_oracle ((spec ++ spec') ++ spec'') (spec' ++ spec''') :=
+-- (so ++ₛ so') +++ₛ so''
 
 variables (so : simulation_oracle spec spec'') (so' : simulation_oracle spec' spec'')
   (i : spec.ι) (i' : spec'.ι) (t : spec.domain i) (t' : spec'.domain i')
